checkpoint

examples/dsls/bool_refinement/BoolRefinement.fst
@@ -1,15 +1,13 @@
-module STLC
+module BoolRefinement
 module T = FStar.Tactics
 module R = FStar.Reflection
 module L = FStar.List.Tot
-
 
 let var = nat
 let index = nat
 
 let tun = R.pack_ln R.Tv_Unknown
 
-noeq
 type src_exp =
   | EBVar : index -> src_exp
   | EVar  : var -> src_exp
@@ -40,14 +38,21 @@ let rec ln' (e:src_exp) (n:int)
     | EVar _ -> true
     | EBVar m -> m <= n
     | EIf b e1 e2 -> ln' b n && ln' e1 n && ln' e2 n
-    | ELam _ e -> ln' e (n + 1)
+    | ELam t e -> ln_ty t && ln' e (n + 1)
     | EApp e1 e2 -> ln' e1 n && ln' e2 n
+and ln_ty (e:src_ty )
+  : bool
+  = match e with
+    | TBool -> true
+    | TRefineBool e -> ln' e (- 1)
+    | TArrow t1 t2 -> ln_ty t1 && ln_ty t2
 
 let ln e = ln' e (-1)
 
+
 let rec open_exp' (e:src_exp) (v:var) (n:index)
   : e':src_exp { size e == size e'}
-  = match e with
+    = match e with
     | EBool _ -> e
     | EVar m -> EVar m
     | EBVar m -> if m = n then EVar v else EBVar m
@@ -125,60 +130,69 @@ let rec close_exp_ln (e:src_exp) (v:var) (n:nat)
     | EApp e1 e2 -> close_exp_ln e1 v n; close_exp_ln e2 v n
 
 
-let src_env = list (either (var & src_ty)      //either a type binding
-                           (src_exp & src_exp) //or an equation between two src exps
-                           )
+let src_eqn = src_exp & src_exp
 
-let rec lookup (e:src_env) (x:var)
-  : option src_ty
+//environment binds types or equations
+let src_env = list (var & either src_ty src_eqn) 
+
+let rec lookup (e:list (var & 'a)) (x:var)
+  : option 'a
   = match e with
     | [] -> None
-    | Inl (y, t) :: tl -> if x = y then Some t else lookup tl x
-    | Inr _ :: tl -> lookup tl x
+    | (y, v) :: tl -> if x = y then Some v else lookup tl x
 
+let lookup_ty (e:src_env) (x:var)
+  : option src_ty
+  = match lookup e x with
+    | Some (Inl t) -> Some t
+    | _ -> None
+    
 let max (n1 n2:nat) = if n1 < n2 then n2 else n1
 
-let rec fresh (e:src_env)
+let rec fresh (e:list (var & 'a))
   : var
   = match e with
     | [] -> 0
-    | Inl (y, _) :: tl ->  max (fresh tl) y + 1
+    | (y, _) :: tl ->  max (fresh tl) y + 1
     | _ :: tl -> fresh tl
 
-// let rec fresh_not_mem (e:list (var & 'a)) (elt: (var & 'a))
-//   : Lemma (ensures L.memP elt e ==> fresh e > fst elt)
-//   = match e with
-//     | [] -> ()
-//     | hd :: tl -> fresh_not_mem tl elt
+let rec fresh_not_mem (e:list (var & 'a)) (elt: (var & 'a))
+  : Lemma (ensures L.memP elt e ==> fresh e > fst elt)
+  = match e with
+    | [] -> ()
+    | hd :: tl -> fresh_not_mem tl elt
   
-// let rec lookup_mem (e:list (var & 'a)) (x:var)
-//   : Lemma
-//     (requires Some? (lookup e x))
-//     (ensures exists elt. L.memP elt e /\ fst elt == x)
-//   = match e with
-//     | [] -> ()
-//     | hd :: tl -> 
-//       match lookup tl x with
-//       | None -> assert (L.memP hd e)
-//       | _ -> 
-//         lookup_mem tl x;
-//         eliminate exists elt. L.memP elt tl /\ fst elt == x
-//         returns _
-//         with _ . ( 
-//           introduce exists elt. L.memP elt e /\ fst elt == x
-//           with elt
-//           and ()
-//         )
+let rec lookup_mem (e:list (var & 'a)) (x:var)
+  : Lemma
+    (requires Some? (lookup e x))
+    (ensures exists elt. L.memP elt e /\ fst elt == x)
+  = match e with
+    | [] -> ()
+    | hd :: tl -> 
+      match lookup tl x with
+      | None -> assert (L.memP hd e)
+      | _ -> 
+        lookup_mem tl x;
+        eliminate exists elt. L.memP elt tl /\ fst elt == x
+        returns _
+        with _ . ( 
+          introduce exists elt. L.memP elt e /\ fst elt == x
+          with elt
+          and ()
+        )
 
 let fresh_is_fresh (e:src_env)
   : Lemma (None? (lookup e (fresh e)))
-  = admit()
+  =  match lookup e (fresh e) with
+     | None -> ()
+     | Some _ ->
+       lookup_mem e (fresh e);
+       FStar.Classical.forall_intro (fresh_not_mem e)
 
 [@@erasable]
 noeq
 type sub_typing : src_env -> src_ty -> src_ty -> Type =
   | S_Refl : g:src_env -> t:src_ty -> sub_typing g t t
-  
 
 [@@erasable]
 noeq
@@ -190,8 +204,8 @@ type src_typing : src_env -> src_exp -> src_ty -> Type =
   
   | T_Var  :
       g:src_env ->
-      x:var { Some? (lookup g x) } ->
-      src_typing g (EVar x) (Some?.v (lookup g x))
+      x:var { Some? (lookup_ty g x) } ->
+      src_typing g (EVar x) (Some?.v (lookup_ty g x))
 
   | T_Lam  :
       g:src_env ->
@@ -200,7 +214,7 @@ type src_typing : src_env -> src_exp -> src_ty -> Type =
       t':src_ty ->
       x:var { x == fresh g } ->
       src_ty_ok g t ->
-      src_typing (Inl(x,t)::g) (open_exp e x) t' ->
+      src_typing ((x, Inl t) :: g) (open_exp e x) t' ->
       src_typing g (ELam t e) (TArrow t t')
 
   | T_App  :
@@ -224,8 +238,8 @@ type src_typing : src_env -> src_exp -> src_ty -> Type =
        t2:src_ty ->
        t:src_ty ->
        src_typing g b TBool ->
-       src_typing (Inr (b, EBool true) :: g) e1 t1 ->
-       src_typing (Inr (b, EBool false) :: g) e2 t2 ->
+       src_typing ((fresh g, Inr (b, EBool true)) :: g) e1 t1 ->
+       src_typing ((fresh g, Inr (b, EBool false)) :: g) e2 t2 ->
        sub_typing g t1 t ->
        sub_typing g t2 t ->
        src_typing g (EIf b e1 e2) t
@@ -240,7 +254,20 @@ and src_ty_ok : src_env -> src_ty -> Type =
                 e:src_exp ->
                 src_typing [] e (TArrow TBool TBool) ->
                 src_ty_ok g (TRefineBool e)
-                                      
+
+let check_sub_typing (g:R.env) 
+                     (sg:src_env)
+                     (t0 t1:src_ty)
+  : T.Tac (sub_typing sg t0 t1)
+  = if t0 = t1 then S_Refl _ t0
+    else T.fail "Not subtypes"
+
+let weaken (g:R.env) (sg:src_env) (t0 t1:src_ty)
+  : T.Tac (t:src_ty & sub_typing sg t0 t & sub_typing sg t1 t)
+  = if t0 = t1
+    then (| t0, S_Refl _ t0, S_Refl _ t1 |)
+    else T.fail "weaken is very dumb"
+  
 let rec check (g:R.env)
               (sg:src_env)
               (e:src_exp { ln e })
@@ -253,67 +280,78 @@ let rec check (g:R.env)
 
     | EVar n ->
       begin
-      match lookup sg n with
+      match lookup_ty sg n with
       | None -> T.fail "Ill-typed"
       | Some t ->
         let d = T_Var sg n in
         (| EVar n, t, d |)
       end
 
-    | _ -> admit()
     | ELam t e ->
+      let (| t, t_ok |) = check_ty g sg t in
       let x = fresh sg in
       fresh_is_fresh sg;
-      let t = read_back g rt in
-      let (| e, tbody, dbody |) = check g ((x,t)::sg) (open_exp e x) in
+      let (| e, tbody, dbody |) = check g ((x, Inl t)::sg) (open_exp e x) in
       (| ELam t (close_exp e x), 
          TArrow t tbody, 
-         T_Lam sg t (close_exp e x) tbody x dbody |)
-           
+         T_Lam sg t (close_exp e x) tbody x t_ok dbody |)
+
     | EApp e1 e2 ->
       let (| e1, t1, d1 |) = check g sg e1  in
       let (| e2, t2, d2 |) = check g sg e2 in
+      begin
       match t1 with
-      | TArrow t2' t ->
-        if t2' = t2
-        then (| EApp e1 e2, t, T_App _ _ _ _ _ d1 d2 |)
-        else T.fail "Inference went wrong"
-        
-      | _ -> 
-        T.fail "Inference went wrong"
+      | TArrow t_arg t_res ->
+        let st_ok = check_sub_typing g sg t2 t_arg in
+        (| EApp e1 e2, t_res, T_App _ _ _ t_arg t_res _ d1 d2 st_ok |)
 
-let infer_and_check (g:R.env)
-                    (e:stlc_exp unit { ln e })
-  : T.Tac (e':s_exp { ln e' } &
-           t :stlc_ty { stlc_typing [] e' t })
-  = let (| e', _ |) = infer g [] e in
-    let (| e'', t', d |) = check g [] e' in
-    (| e'', t' |)
+      | _ -> 
+        T.fail "Expected a function"
+      end
+
+    | EIf b e1 e2 ->
+      let (| b, tb, ok_b |) = check g sg b in
+      let hyp = fresh sg in
+      if tb = TBool
+      then (
+        let (| e1, t1, ok_1 |) = check g ((hyp, Inr(b, EBool true))::sg) e1 in
+        let (| e2, t2, ok_2 |) = check g ((hyp, Inr(b, EBool false))::sg) e2 in      
+        let (| t, w1, w2 |) = weaken g sg t1 t2 in
+        (| EIf b e1 e2, t, T_If _ _ _ _ _ _ _ ok_b ok_1 ok_2 w1 w2 |)
+      )
+      else T.fail "Branching on a non-boolean"
+
+and check_ty (g:R.env)
+             (sg:src_env)
+             (t:src_ty{ln_ty t})
+  : T.Tac (t':src_ty { ln_ty t' } &
+           src_ty_ok sg t')
+  = match t with
+    | TBool -> (| t, OK_TBool _ |)
+
+    | TArrow t t' ->
+      let (| t, t_ok |) = check_ty g sg t in
+      let (| t', t'_ok |) = check_ty g sg t' in      
+      (| TArrow t t', OK_TArrow _ _ _ t_ok t'_ok |)
+      
+    | TRefineBool e ->
+      let (| e, te, de |) = check g [] e in
+      match te with
+      | TArrow TBool TBool -> (| TRefineBool e, OK_Refine _ _ de |)
+      | _ -> T.fail "Ill-typed refinement"
+  
 
 module RT = Refl.Typing
 
-let rec elab_ty (t:stlc_ty) 
-  : R.term 
-  = let open R in
-    match t with
-    | TUnit -> 
-      R.pack_ln (R.Tv_FVar (R.pack_fv unit_lid))
-      
-    | TArrow t1 t2 ->
-      let t1 = elab_ty t1 in
-      let t2 = elab_ty t2 in
-
-      R.pack_ln 
-        (R.Tv_Arrow 
-          (RT.as_binder 0 t1)
-          (R.pack_comp (C_Total t2 [])))
-  
-let rec elab_exp (e:s_exp)
-  : Tot R.term (decreases (size e))
+let rec elab_exp (e:src_exp)
+  : Tot R.term
   = let open R in
     match e with
-    | EUnit -> 
-      pack_ln (Tv_Const C_Unit)
+    | EBool true ->
+      pack_ln (Tv_Const R.C_True)
+
+    | EBool false ->
+      pack_ln (Tv_Const R.C_False)
 
     | EBVar n -> 
       let bv = R.pack_bv (RT.make_bv n tun) in
@@ -334,15 +372,59 @@ let rec elab_exp (e:s_exp)
       let e2 = elab_exp e2 in
       R.pack_ln (Tv_App e1 (e2, Q_Explicit))
 
-let extend_env_l (g:R.env) (sg:stlc_env) = 
-  L.fold_right (fun (x, t) g -> RT.extend_env g x (elab_ty t)) sg g
-  
-let rec extend_env_l_lookup_bvar (g:R.env) (sg:stlc_env) (x:var)
+    | EIf b e1 e2 ->
+      let b = elab_exp b in
+      let e1 = elab_exp e1 in
+      let e2 = elab_exp e2 in
+      R.pack_ln (Tv_Match b None [(Pat_Constant C_True, e1); (Pat_Constant C_False, e2)])
+      
+and elab_ty (t:src_ty) 
+  : R.term  
+  = let open R in
+    match t with
+    | TBool -> 
+      RT.bool_ty
+      
+    | TArrow t1 t2 ->
+      let t1 = elab_ty t1 in
+      let t2 = elab_ty t2 in
+      R.pack_ln 
+        (R.Tv_Arrow 
+          (RT.as_binder 0 t1)
+          (R.pack_comp (C_Total t2 [])))
+          
+    | TRefineBool e ->
+      let e = elab_exp e in
+      let bv = R.pack_bv (RT.make_bv 0 RT.bool_ty) in
+      let refinement = R.pack_ln (Tv_App e (R.pack_ln (Tv_BVar bv), Q_Explicit)) in
+      R.pack_ln (Tv_Refine bv refinement)
+
+module F = FStar.Reflection.Formula
+let elab_eqn (e1 e2:src_exp)
+  : R.term
+  =  F.formula_as_term (F.Comp (F.Eq (Some RT.bool_ty))
+                                     (elab_exp e1)
+                                     (elab_exp e2))
+
+let binding = either src_ty src_eqn
+let elab_binding (b:binding)
+  : R.term 
+  = match b with
+    | Inl t -> elab_ty t
+    | Inr (e1, e2) -> elab_eqn e1 e2
+    
+let extend_env_l (g:R.env) (sg:src_env) = 
+  L.fold_right 
+    (fun (x, b) g ->  RT.extend_env g x (elab_binding b))
+     sg
+     g
+
+let rec extend_env_l_lookup_bvar (g:R.env) (sg:src_env) (x:var)
   : Lemma 
     (requires (forall x. RT.lookup_bvar g x == None))
     (ensures (
       match lookup sg x with
-      | Some t -> RT.lookup_bvar (extend_env_l g sg) x == Some (elab_ty t)
+      | Some b -> RT.lookup_bvar (extend_env_l g sg) x == Some (elab_binding b)
       | None -> RT.lookup_bvar (extend_env_l g sg) x == None))
     (decreases sg)
     [SMTPat (RT.lookup_bvar (extend_env_l g sg) x)]
@@ -350,40 +432,75 @@ let rec extend_env_l_lookup_bvar (g:R.env) (sg:stlc_env) (x:var)
     | [] -> ()
     | hd :: tl -> extend_env_l_lookup_bvar g tl x
 
-let elab_open_commute (e:s_exp) (x:var)
+let elab_open_commute (e:src_exp) (x:var)
   : Lemma (RT.open_term (elab_exp e) x == elab_exp (open_exp e x))
           [SMTPat (RT.open_term (elab_exp e) x)]
   = admit()
 
 //key lemma about STLC types
-let stlc_types_are_closed1 (ty:stlc_ty) (v:R.term)
+let src_types_are_closed1 (ty:src_ty) (v:R.term)
   : Lemma (RT.open_with (elab_ty ty) v == elab_ty ty)
-          [SMTPat (RT.open_with (elab_ty ty) v)]
+//          [SMTPat (RT.open_with (elab_ty ty) v)]
   = admit()
 
-let stlc_types_are_closed2 (ty:stlc_ty) (x:R.var)
+let src_types_are_closed2 (ty:src_ty) (x:R.var)
   : Lemma (RT.close_term (elab_ty ty) x == elab_ty ty)
           [SMTPat (RT.close_term (elab_ty ty) x)]
   = admit()
 
-let rec soundness (#sg:stlc_env) 
-                  (#se:s_exp)
-                  (#st:stlc_ty)
-                  (dd:stlc_typing sg se st)
-                  (g:R.env { forall x. None? (RT.lookup_bvar g x) } )
+
+let stlc_types_are_closed3 (ty:src_ty) (x:R.var)
+  : Lemma (RT.open_term (elab_ty ty) x == elab_ty ty)
+          [SMTPat (RT.open_term (elab_ty ty) x)]
+  = admit()
+
+let fstar_env =
+  g:R.env { 
+    RT.lookup_fvar g RT.bool_fv == Some RT.tm_type
+  }
+
+let fstar_top_env =
+  g:fstar_env { 
+    forall x. None? (RT.lookup_bvar g x )
+  }
+
+let extend_env_l_lookup_fvar (g:R.env) (sg:src_env) (fv:R.fv)
+  : Lemma 
+    (ensures
+      RT.lookup_fvar (extend_env_l g sg) fv ==
+      RT.lookup_fvar g fv)
+    [SMTPat (RT.lookup_fvar (extend_env_l g sg) fv)]
+  = admit()
+
+let src_ty_ok_weakening (sg:src_env) 
+                        (x:var { None? (lookup sg x) })
+                        (b:binding)
+                        (t:src_ty)
+                        (d:src_ty_ok sg t)
+  : GTot (src_ty_ok ((x, b)::sg) t)
+  = admit()
+                        
+let rec soundness (#sg:src_env) 
+                  (#se:src_exp)
+                  (#st:src_ty)
+                  (dd:src_typing sg se st)
+                  (g:fstar_top_env)
   : GTot (RT.typing (extend_env_l g sg)
                     (elab_exp se)
                     (elab_ty st))
          (decreases dd)
   = match dd with
-    | T_Unit _ ->
-      RT.T_Const _
+    | T_Bool _ true ->
+      RT.T_Const _ _ _ RT.CT_True
+
+    | T_Bool _ false ->
+      RT.T_Const _ _ _ RT.CT_False
 
     | T_Var _ x ->
       RT.T_Var _ (R.pack_bv (RT.make_bv x tun))
 
-    | T_Lam _ t e t' x de ->
-      let de : RT.typing (extend_env_l g ((x,t)::sg))
+    | T_Lam _ t e t' x dt de ->
+      let de : RT.typing (extend_env_l g ((x,Inl t)::sg))
                          (elab_exp (open_exp e x))
                          (elab_ty t')
             = soundness de g 
@@ -394,6 +511,9 @@ let rec soundness (#sg:stlc_env)
              = de
       in
       fresh_is_fresh sg;
+      let dt : RT.typing (extend_env_l g sg) (elab_ty t) RT.tm_type =
+        src_ty_ok_soundness g sg t dt
+      in
       let dd
         : RT.typing (extend_env_l g sg)
                     (R.pack_ln (R.Tv_Abs (RT.as_binder 0 (elab_ty t)) (elab_exp e)))
@@ -403,9 +523,31 @@ let rec soundness (#sg:stlc_env)
                    (elab_ty t) 
                    (elab_exp e)
                    (elab_ty t')
+                   dt
                    de
       in
       dd
+
+    | _ -> admit()
+
+and src_ty_ok_soundness (g:fstar_top_env)
+                        (sg:src_env)
+                        (t:src_ty)
+                        (dt:src_ty_ok sg t)
+ : GTot (RT.typing (extend_env_l g sg) (elab_ty t) RT.tm_type)
+        (decreases t)
+ = match dt with
+   | OK_TBool _ -> RT.T_FVar _ RT.bool_fv
+   | OK_TArrow _ t1 t2 ok_t1 ok_t2 ->
+     let t1_ok = src_ty_ok_soundness g sg _ ok_t1 in
+     let x = fresh sg in
+     fresh_is_fresh sg;
+     let t2_ok = src_ty_ok_soundness g ((x, Inl t1)::sg) _ (src_ty_ok_weakening _ _ _ _ ok_t2) in
+     RT.T_Arrow _ x (elab_ty t1) (elab_ty t2) t1_ok t2_ok
+     
+   | _ -> admit()
+
+
 
     | T_App _ e1 e2 t t' d1 d2 ->
       let dt1 
