examples/dsls/core/Refl.Typing.fsti
@@ -49,9 +49,22 @@ let binder_sort_lemma (x:var) (ty:term)
           [SMTPat (binder_sort (as_binder x ty))]
   = admit()          
 
-let unit_exp = pack_ln (Tv_Const C_Unit)
-let unit_ty = pack_ln (Tv_FVar (pack_fv unit_lid))
+let constant_as_term (v:vconst) = pack_ln (Tv_Const v)
+let unit_exp = constant_as_term C_Unit
+let unit_fv = pack_fv unit_lid
+let unit_ty = pack_ln (Tv_FVar unit_fv)
+let bool_fv = pack_fv bool_lid
+let bool_ty = pack_ln (Tv_FVar bool_fv)
 
+let mk_total t = pack_comp (C_Total t [])
+let tm_type = pack_ln (Tv_Type ())
+
+noeq
+type constant_typing: vconst -> term -> Type0 = 
+  | CT_Unit: constant_typing C_Unit unit_ty
+  | CT_True: constant_typing C_True bool_ty
+  | CT_False: constant_typing C_False bool_ty  
+  
 noeq
 type typing : env -> term -> term -> Type0 =
   | T_Var : 
@@ -59,9 +72,17 @@ type typing : env -> term -> term -> Type0 =
      x:bv { Some? (lookup_bvar g (bv_index x)) } ->
      typing g (pack_ln (Tv_Var x)) (Some?.v (lookup_bvar g (bv_index x)))
 
+  | T_FVar :
+     g:env ->
+     x:fv { Some? (lookup_fvar g x) } -> 
+     typing g (pack_ln (Tv_FVar x)) (Some?.v (lookup_fvar g x))
+     
   | T_Const:
      g:env ->
-     typing g unit_exp unit_ty
+     v:vconst ->
+     t:term ->
+     constant_typing v t ->
+     typing g (constant_as_term v) t
 
   | T_Abs :
      g:env ->
@@ -69,10 +90,11 @@ type typing : env -> term -> term -> Type0 =
      ty:term ->
      body:term ->
      body_ty:term ->
+     typing g ty tm_type ->
      typing (extend_env g x ty) (open_term body x) body_ty ->
      typing g (pack_ln (Tv_Abs (as_binder 0 ty) body))
               (pack_ln (Tv_Arrow (as_binder 0 ty) 
-                                 (pack_comp (C_Total (close_term body_ty x) []))))
+                                 (mk_total (close_term body_ty x))))
 
   | T_App :
      g:env ->
@@ -84,3 +106,13 @@ type typing : env -> term -> term -> Type0 =
      typing g e2 (binder_sort x) ->
      typing g (pack_ln (Tv_App e1 (e2, Q_Explicit)))
               (open_with t e2)
+
+  | T_Arrow:
+     g:env ->
+     x:var { None? (lookup_bvar g x) } ->
+     t1:term ->
+     t2:term ->
+     typing g t1 tm_type ->
+     typing (extend_env g x t1) (open_term t2 x) tm_type ->
+     typing g (pack_ln (Tv_Arrow (as_binder 0 t1) (mk_total t2))) tm_type
+     
